makefile
@@ -3,4 +3,4 @@ DATE=`date +'%d/%m/%y'`
 eod:
 	git add -A ; \
 	git commit -m "end of day $(DATE)" ; \
-	git push origin inference ; \
+	git push origin $(BRANCH) ; \
